---
title: Hodge theory on compact hermitian manifolds - 3
date: 2025-07-14 14:12:00
tags:
	- complex geometry
	- math
mathjax: true
---

The proof of *Theorem A* and *Theorem C* appeared in the previous post will be given in this one. Note that the standard Rellich lemma in functional analysis will be applied without a proof. 

We always suppose that $M$ is a compact hermitian manifold and $E$ is a holomorphic vector bundle on $M$ endowed with a hermitian metric $h$. 

## Theorem A

Recall that the hermitian structures on $M$ and $E$ induce an inner product on the space $A(M,E)$, and hence the norms $\\\|\cdot\\\|\_s$ on $A(M,E)$ given by $$\\\|\xi\\\|\_s^2 = \sum_{k=0}^s \\\|\nabla^k\xi\\\|^2 = \sum_{k=0}^s (\nabla^k\xi, \nabla^k\xi), \quad \xi \in A(M,E),$$ where $\nabla$ is the metric connection on $E$ with respect to $h$. Considering the completion of $A(M,E)$ with respect to $\\\|\cdot\\\|\_s$ and its dual space, we obtain the Sobolev spaces $H_s(M,E)$ and $H_{-s}(M,E)$. The operators $\bar{\partial}, \bar{\partial}^\*$ and $\nabla$ on $A(M,E)$ extends to differential operators of order one from $H_s(M,E)$ to $H_{s-1}(M,E)$, while $\Delta$ becomes differential operators of order two from $H_s(M,E)$ to $H_{s-2}(M,E)$. 

The statement of *Theorem A* is the following. 

**Theorem A (G&#229;rding's inequality).** There exist positive constants $c_1, c_2 > 0$ such that for each $\xi \in A(M, E)$, we have $$(\Delta\xi, \xi) \geq c_1 \\\|\xi\\\|_1^2 - c_2 \\\|\xi\\\|_0^2.$$

---

To prove *Theorem A*, we need to estimate the lower bound of $(\Delta\xi,\xi)$. The compactness of $M$ suggests that we can process the estimation locally. First introduce some notations. Suppose $v_1, \cdots, v_n$ form a local orthonormal frame of $T^{1,0}(M)$ with dual frame $\\\{\varphi^1, \cdots, \varphi^n\\\}$. Let $\\\{e^1, \cdots, e^r\\\}$ be a local holomorphic frame of $E$, whose dual frame of $E^\*$ is given by $\\\{e^\*\_1, \cdots, e^\*\_r\\\}$. Then an $E$-valued form $\xi \in A^{p,q}(M,E)$ can be expressed by $$\xi = \sum\_{I,J,k} \xi_{I\bar{J}k} \\\, \varphi^I \wedge \bar{\varphi}^J \otimes e^k,$$ where the summation is taken over subsets $I$ and $J$ of $\\\{1, \cdots, n\\\}$ with $|I| = p$ and $|J| = q$. For a local smooth function $f$, denote that $$f_j = v_j f, \quad f_\bar{j} = \bar{v}\_j f, \quad j = 1, \cdots, n.$$ We can see that $$\partial f = \sum_{j=1}^n f_j \varphi^j, \quad \bar{\partial}f = \sum_{j=1}^n f\_\bar{j} \bar{\varphi}^j.$$ However, in general we do not have $$\bar{\partial}\xi = \sum_{I,J,k} \sum_{j=1}^n \xi_{I\bar{J}k,\bar{j}} \\\, \bar{\varphi}^j \wedge \varphi^I \wedge \bar{\varphi}^J \otimes e^k.$$ Indeed, it should be $$\bar{\partial}\xi = \sum\_{I,J,k} \bar{\partial}\left(\xi_{I\bar{J}k} \\\, \varphi^I \wedge \bar{\varphi}^J\right) \otimes e^k = \sum\_{I,J,k} \left(\bar{\partial}\xi_{I\bar{J}k} \wedge \varphi^I \wedge \bar{\varphi}^J + \xi_{I\bar{J}k} \\\, \bar{\partial}\left(\varphi^I \wedge \bar{\varphi}^J\right)\right) \otimes e^k = \sum_{I,J,k} \sum_{j=1}^n \xi_{I\bar{J}k,\bar{j}} \\\, \bar{\varphi}^j \wedge \varphi^I \wedge \bar{\varphi}^J \otimes e^k + P^0(\xi),$$ where we use $P^0(\xi)$ to denote a term containing only $\xi_{I\bar{J}k}$ instead of any derivative of them. The specific expression of $P^0(\xi)$ is of no importance as we just need to know that it can be bounded by some multiple of $\\\|\xi\\\|\_0$ in our estimation. Similarly we can denote by $P^t(\xi)$ the terms only containing the derivatives of $\xi\_{I\bar{J}k}$ of order no more than $t$ and hence dominated by $\\\|\xi\\\|\_t$. An example is that $$f_{jk} - f_{kj} = v_k v_j f - v_j v_k f = [v_k, v_j]f = P^1(f),$$ which permits us to ignore the ordering of partial differentiations up to lower-order terms. 

---

**Lemma (Weitzenb&#246;ck formula).** Suppose $\xi \in A(M,E)$ is given locally as $$\xi = \sum\_{I,J,k} \xi_{I\bar{J}k} \\\, \varphi^I \wedge \bar{\varphi}^J \otimes e^k.$$ Then $$\Delta\xi = -2\sum_{I,J,k} \sum_{j=1}^n \xi_{I\bar{J}k,j\bar{j}} \\\, \varphi^I \wedge \bar{\varphi}^J \otimes e^k + P^1(\xi).$$

> *Proof:* Clearly we can reduce the assertion to $\xi \in A^{p,q}(M,E)$. We claim that this can further reduce to $\alpha \in A^{p,q}(M)$. Let $h^{j\bar{k}} = h(e^j, e^k)$ for $j,k = 1, \cdots, r$. Consider the following computations: $$\bar{\partial}^\*\left(\sum_{k=1}^r \alpha_k \otimes e^k\right) = -\sum_{k=1}^r \*\bar{\partial}\*(\alpha_k \otimes e^k) = -\sum_{k,l=1}^r \*\bar{\partial}(\*\alpha_k \otimes h^{l\bar{k}}e^\*\_l) = -\sum\_{k,l=1}^r \*(\bar{\partial}\*\alpha_k \otimes h^{l\bar{k}}e^\*_l + \bar{\partial}h^{l\bar{k}} \wedge \*\alpha_k \otimes e^\*\_l) = \sum\_{k=1}^r \left(\bar{\partial}^\*\alpha_k \otimes e^k + P^0(\alpha_k)\right).$$ 
> 
> Thus for $$\xi = \sum_{k=1}^r \alpha_k \otimes e^k,$$ we have $$\Delta\xi = \bar{\partial}\left(\sum_{k=1}^r \bar{\partial}^\* \alpha_k \otimes e^k + P^0(\xi)\right) + \bar{\partial}^\*\left(\sum_{k=1}^r \bar{\partial}\alpha_k \otimes e^k\right) = \left(\sum_{k=1}^r \bar{\partial}\bar{\partial}^\*\alpha_k \otimes e^k + P^1(\xi)\right) + \sum_{k=1}^r \left(\bar{\partial}^\*\bar{\partial}\alpha_k \otimes e^k + P^0(\bar{\partial}\alpha_k)\right) = \sum_{k=1}^r \Delta\alpha_k \otimes e^k + P^1(\xi).$$ This proves our assertion. 
>
> Now it remains to show for $$\alpha = \sum_{I,J} \alpha_{I\bar{J}} \\\, \varphi^I \wedge \bar{\varphi}^J \in A^{p,q}(M)$$ that $$\Delta\alpha = -2 \sum_{I,J} \sum_{k=1}^r \alpha_{I\bar{J},k\bar{k}} \\\, \varphi^I \wedge \bar{\varphi}^J + P^1(\alpha).$$ By linearility, we may drop the summation for $I$ and $J$, and as $\bar{\partial}$ and $\bar{\partial}^\*$ have nothing to do with $\varphi^I$, we can assume that $p=0$. The symmetry in the indices further implies that there is no loss of generality assuming that $J = \\\{1, \cdots, q\\\}$. So we only have to deal with $$\alpha = f \\\, \bar{\varphi}^1 \wedge \cdots \wedge \bar{\varphi}^q.$$ 
> 
> Direct computation yields that $$\*\bar{\partial}\*\bar{\partial}\alpha = 2 \sum_{k>q} f_{\bar{k}k} \\\,\bar{\varphi}^1 \wedge \cdots \wedge \bar{\varphi}^q + 2 \sum_{l \leq q < k} (-1)^{l+q-1} f_{\bar{k}l} \\\,\bar{\varphi}^1 \wedge \cdots \wedge \hat{\bar{\varphi}}^l \wedge \cdots \wedge \bar{\varphi}^q \wedge \bar{\varphi}^k + P^1(\alpha),$$ and that $$\bar{\partial}\*\bar{\partial}\*\alpha = 2 \sum_{l \leq q} f_{l\bar{l}} \\\,\bar{\varphi}^1 \wedge \cdots \wedge \bar{\varphi}^q + 2 \sum_{l \leq q < k} (-1)^{l+q} f_{l\bar{k}} \\\,\bar{\varphi}^1 \wedge \cdots \wedge \hat{\bar{\varphi}}^l \wedge \cdots \wedge \bar{\varphi}^q \wedge \bar{\varphi}^k + P^1(\alpha).$$ As $f_{\bar{k}l} - f_{l\bar{k}} = P^1(f)$ for each $k$ and $l$, we obtain $$\Delta\alpha = -\*\bar{\partial}\*\bar{\partial}\alpha - \bar{\partial}\*\bar{\partial}\*\alpha = -2 \sum_{k=1}^r f_{k\bar{k}} \\\, \bar{\varphi}^1 \wedge \cdots \wedge \bar{\varphi}^q + P^1(\alpha),$$ which completes our proof. 

Now we can write down the proof of *Theorem A*. 

> *Proof of Theorem A:* As $A^{p,q}(M,E)$ are orthogonal to each other, it suffices to show the assertion for $\xi \in A^{p,q}(M,E)$ where $p$ and $q$ are fixed. By the definition of the action of $\nabla$ on $A^{p,q}(M,E)$, we see that $\nabla$ is decomposed into $\nabla = \nabla^{1,0} + \nabla^{0,1}$ with $$\nabla^{1,0} : A^{p,q}(M,E) \to A^{p+1,q}(M,E), \quad \nabla^{0,1} : A^{p,q}(M,E) \to A^{p,q+1}(M,E).$$ Moreover, using the local expression of $\xi$ as $$\xi = \sum_{I,J,k} \xi_{I\bar{J}k} \\\, \varphi^I \wedge \bar{\varphi}^J \otimes e^k,$$ we see that $$\nabla^{1,0}\xi = \sum_{I,J,k} \sum_{j=1}^n \xi_{I\bar{J}k,j} \\\, \varphi^j \wedge \varphi^I \wedge \bar{\varphi}^J \otimes e^k + P^0(\xi),$$ and that $$\nabla^{0,1}\xi = \sum_{I,J,k} \sum_{j=1}^n \xi_{I\bar{J}k,\bar{j}} \\\, \bar{\varphi}^j \wedge \varphi^I \wedge \bar{\varphi}^J \otimes e^k + P^0(\xi).$$
>
> Consider the $(n-1,n)$-form $$\psi = (-1)^{n(n-1)/2}\left(\frac{i}{2}\right)^n \sum_{I,J,k,l}\sum_{j=1}^n (-1)^{j-1}h^{k\bar{l}}\\\,\xi_{I\bar{J}k,\bar{j}}\\\,\overline{\xi_{I\bar{J}l}} \\\, \varphi^1 \wedge \cdots \wedge \hat{\varphi}^j \wedge \cdots \wedge \varphi^n \wedge \bar{\varphi}^1 \wedge \cdots \wedge \bar{\varphi}^n,$$ which can be verified to be well-defined (up to some $P^0(\xi)$) globally on the whole $M$. Since $\psi$ is of type $(n-1,n)$, we have $\bar{\partial}\psi = 0$, and then the Stokes' formula implies that $$\int_M \partial\psi = \int_M \mathrm{d}\psi = 0.$$ Direct computation yields that $$\partial\psi = \sum_{I,J,k,l}\sum_{j=1}^n h^{k\bar{l}}\left(\xi_{I\bar{J}k,j\bar{j}}\\\,\overline{\xi_{I\bar{J}l}} + \xi_{I\bar{J}k,\bar{j}}\\\,\overline{\xi_{I\bar{J}l,\bar{j}}}\right) \\\,\mathrm{d}V + \langle P^1(\xi),\xi \rangle \cdot \mathrm{d}V,$$ and then by the Weitzenb&#246;ck formula and the local expression of $\nabla^{0,1}\xi$ we see that $$(\Delta\xi, \xi) - (\nabla^{0,1}\xi, \nabla^{0,1}\xi) + (P^1(\xi),\xi) = 0.$$ Note the inequality $$2|(P^1(\xi),\xi)| \leq \varepsilon\\\|P^1(\xi)\\\|^2 + \frac{1}{\varepsilon}\\\|\xi\\\|^2 \leq \varepsilon C_1 \\\|\xi\\\|_1^2 + \frac{1}{\varepsilon}\\\|\xi\\\|_0^2,$$ we obtain $$\\\|\nabla^{0,1}\xi\\\|^2 \leq (\Delta\xi, \xi) + \frac{\varepsilon C_1}{2}\\\|\xi\\\|_1^2 + \frac{1}{2\varepsilon}\\\|\xi\\\|_0^2.$$ 
> 
> Analogously, consider $$\gamma = (-1)^{n(n+1)/2}\left(\frac{i}{2}\right)^n \sum_{I,J,k,l}\sum_{j=1}^n (-1)^{p+j-1}h^{k\bar{l}}\\\,\xi_{I\bar{J}k,j}\\\,\overline{\xi_{I\bar{J}l}} \\\, \varphi^1 \wedge \varphi^n \wedge \bar{\varphi}^1 \wedge \cdots \wedge \hat{\bar{\varphi}}^j \wedge \cdots \wedge \bar{\varphi}^n,$$ we have $$\\\|\nabla^{1,0}\xi\\\|^2 \leq (\Delta\xi, \xi) + \frac{\delta C_2}{2}\\\|\xi\\\|_1^2 + \frac{1}{2\delta}\\\|\xi\\\|_0^2.$$ Thus $$\\\|\xi\\\|_1^2 = \\\|\xi\\\|^2 + \\\|\nabla^{0,1}\xi\\\|^2 + \\\|\nabla^{1,0}\xi\\\|^2 \leq 2(\Delta\xi, \xi) + \frac{\varepsilon C_1 + \delta C_2}{2}\\\|\xi\\\|_1^2 + \left(1 + \frac{1}{2\varepsilon} + \frac{1}{2\delta}\right)\\\|\xi\\\|_0^2.$$ Taking sufficiently small $\varepsilon$ and $\delta$, we obtain $$(\Delta\xi, \xi) \geq \left(\frac{1}{2} - \frac{\varepsilon C_1 + \delta C_2}{4}\right) \\\|\xi\\\|_1^2 - \frac{1}{2}\left(1 + \frac{1}{2\varepsilon} + \frac{1}{2\delta}\right)\\\|\xi\\\|_0^2,$$ which is exactly the G&#229;rding's inequality.

## Rellich lemma and Theorem C

Recall our statement of *Theorem C*:

**Theorem C.** Suppose $\\\{\xi_n\\\}$ is a sequence in $A(M,E)$ such that $\\\|\xi_n\\\|\_1$ is bounded. Then there exists a subsequence $\\\{\xi\_{n_k}\\\}$ of $\\\{\xi_n\\\}$ which is a Cauchy sequence with respect to $\\\|\cdot\\\|_0$, i.e., converges in $H_0(M,E)$. 

Let us first consider the local case, which relies on some discussion of Sobolev spaces $H_s(U)$, where $U \subset \mathbb{C}^n = \mathbb{R}^{2n}$ is an open subsets. Recall that $H_s(U)$ with $s \geq 0$ is the completion of $A_s(U)$ with respect to $\\\|\cdot\\\|_s$, where $$A_s(U) = \\\{f \in C^\infty(U) \mid \\\|f\\\|_s < +\infty\\\}.$$ Clearly we have $C^\infty_c(U) \subset A_s(U)$ for any $s \geq 0$, and hence we can consider the closure of $C^\infty_c(U)$ in $H_s(U)$, which is exactly the completion of $C^\infty_c(U)$ with respect to $\\\|\cdot\\\|_s$ and usually denoted by $H^\circ_s(U)$. As we have $H_t(U) \subset H_s(U)$ whenever $0 \leq s < t$, there is a natural inclusion $i : H^\circ_t(U) \to H^\circ_s(U)$.

We have the following result in functional analysis. 

**Theorem (Rellich lemma).** Suppose $U \subset \mathbb{R}^m$ is a bounded open subset and $0 \leq s < t$. Then the natural inclusion $i : H^\circ_t(U) \to H^\circ_s(U)$ is a compact operator. 

Suppose $\\\{U_\alpha\\\}\_{\alpha=1}^l$ is an open cover of $M$ such that on each $U_\alpha$ we have a holomorphic coordinate map and a holomorphic frame $\\\{e^1_\alpha, \cdots, e^r_\alpha\\\}$ of $E$. Suppose $\\\{\eta_\alpha\\\}$ is a smooth partition of unity subordinate to the open cover $\\\{U_\alpha\\\}$. Write for each $\xi \in A(M,E)$ that $$\eta_\alpha \xi = \sum_{I,J,k} \xi^\alpha_{I\bar{J}k} \\\, \mathrm{d}z_\alpha^I \wedge \mathrm{d}\bar{z}\_\alpha^J \otimes e^k_\alpha, \quad \alpha = 1, \cdots, l.$$ We have seen that the norm $\\\|\cdot\\\|_s^\prime$ given by 

$${\\\|\xi\\\|\_s^\prime}^2= \sum_{|\nu| \leq s} \sum_{\alpha=1}^l \sum_{I,J,k} \int\_{U_\alpha} |D^\nu \xi^\alpha_{I\bar{J}k}|^2 \mathrm{d}\mu$$ is equivalent to $\\\|\cdot\\\|_s$. 

> *Proof of Theorem C:* Consider the above open cover $\\\{U_\alpha\\\}$ and $\\\{\eta_\alpha\\\}$. Then each $(\xi_n)^\alpha_{I\bar{J}k}$ is compactly supported on $U_\alpha$, and the sequence $\left\\\{(\xi_n)^\alpha_{I\bar{J}k}\right\\\}\_n$ is bounded in $H^\circ\_1(U_\alpha)$. As $I$, $J$, $k$ and $\alpha$ has only finitely many choices, we obtain from the Rellich lemma that there is a subsequence $\\\{\xi\_{n_t}\\\}$ of $\\\{\xi_n\\\}$ such that $\left\\\{\left(\xi\_{n_t}\right)^\alpha_{I\bar{J}k}\right\\\}$ is Cauchy in $H^\circ\_0(U_\alpha)$. This directly implies that $\\\{\xi\_{n_t}\\\}$ is Cauchy in $H_0(M,E)$ after the equivalence of $\\\|\cdot\\\|_0$ and $\\\|\cdot\\\|_0^\prime$. 