---
title: K&#228;hler manifolds - 2
date: 2025-07-22 21:30:00
tags:
	- complex geometry
	- math
mathjax: true
---

For a complex manifold $M$, we have two different cohomology theory: the de Rham cohomology and the Dolbeault cohomology. As they both come from the cochain of differential forms on $M$, the relations between them are worth considering. In this post we demonstrate this relation on compact K&#228;hler manifolds, which is given by the Hodge decompostion. 

## Fundamental identities

Before the Hodge decompostion, we need some preliminary fundamental identities on K&#228;hler manifolds which are useful not only for the Hodge decompostion in this post but also the Lefschetz decomposition in the next post.

Suppose $M$ is an $n$-dimensional complex manifold with a hermitian metric $h$ and $\omega$ is the associated fundamental form of $h$. The hermitian structure induces a Riemannian structure on $M$, which further induces a volume form $$\mathrm{d}V = \frac{\omega^n}{n!}$$ on $M$ and a star operator $\*$ on the space $A(M)$ of differential forms on $M$ that maps $A^{p,q}(M)$ into $A^{n-p,n-q}(M)$. We have differential operators $\mathrm{d}$, $\partial$ and $\bar{\partial}$ on $M$ which are related by $$\mathrm{d} = \partial + \bar{\partial}, \quad \partial A^{p,q}(M) \subset A^{p+1,q}(M), \quad \bar{\partial} A^{p,q}(M) \subset A^{p,q+1}(M).$$ Consider the operators $$\partial^\* = -\*\partial\*, \quad \bar{\partial}^\* = -\*\bar{\partial}\*.$$ The hermitian structure of $M$ gives an inner product on the space $A_\mathrm{c}^{p,q}(M) \subset A^{p,q}(M)$ consisting of $(p,q)$-form on $M$ with compact support by $$(\alpha, \beta) = \int_M \alpha \wedge \*\beta, \quad \alpha, \beta \in A_\mathrm{c}^{p,q}(M).$$ Then an inner product on $A_\mathrm{c}(M)$ is constructed from these inner products on $A_\mathrm{c}^{p,q}(M)$. With respect to this inner product, it verifies that $\partial$ and $\partial^\*$ are the dual of each other, and $\bar{\partial}$ and $\bar{\partial}^\*$ are the dual of each other. 

Using the fundamental form $\omega$, we can define the **Lefschetz operator** $L : A(M) \to A(M)$ by $$L(\alpha) = \omega \wedge \alpha, \quad \alpha \in A(M).$$ It is direct to see that $L(A^{p,q}(M)) \subset A^{p+1,q+1}(M)$. Define another operator $\Lambda$ on $A(M)$ by $$\Lambda(\alpha) = (-1)^{p+q} \* L \* (\alpha), \quad \alpha \in A^{p,q}(M).$$ We see that $\Lambda$ is exactly the dual of $L$ on $A_\mathrm{c}(M)$ with respect to the inner product $(\cdot,\cdot)$. As $\omega$ is a real form, $L$ and hence $\Lambda$ must be real operators, that is $$L(\bar{\alpha}) = \overline{L(\alpha)}, \quad \Lambda(\bar{\alpha}) = \overline{\Lambda(\alpha)}, \quad \alpha \in A(M).$$ 

---

For two operators $A$ and $B$ on a space, their *commutator* is defined by $$[A,B] = AB - BA.$$

**Proposition.** If $M$ is a K&#228;hler manifold, then it holds on $A(M)$ that $$[\partial,L] = [\bar{\partial},L] = [\partial^\*,\Lambda] = [\bar{\partial}^\*,\Lambda] = 0,$$ i.e., $L$ commutes with $\partial$ and $\bar{\partial}$, and $\Lambda$ commutes with $\partial^\*$ and $\bar{\partial}^\*$. 

> *Proof:* As $M$ is a K&#228;hler form, we have $\mathrm{d}\omega = 0$. Since $\omega$ is a $(1,1)$-form, it follows that $\partial\omega = \bar{\partial}\omega = 0$. Hence for any $\alpha \in A(M,E)$, $$[\partial, L]\alpha = \partial(\omega \wedge \alpha) - \omega \wedge \partial\alpha = \partial\omega \wedge \alpha = 0,$$ $$[\bar{\partial}, L]\alpha = \bar{\partial}(\omega \wedge \alpha) - \omega \wedge \bar{\partial}\alpha = \bar{\partial}\omega \wedge \alpha = 0.$$ Now consier any $\alpha \in A^{p,q}(M)$. We have $$[\partial^\*, \Lambda]\alpha = -(-1)^{p+q}\*\partial\*\* L \*\alpha + (-1)^{p+q-1} \* L \* \* \partial \* \alpha = -\*[\partial,L]\*\alpha = 0,$$ and analogously for $[\bar{\partial}^\*,\Lambda]$.

**Proposition.** For a K&#228;hler manifold $M$, it holds on $A_\mathrm{c}(M)$ that $$[\partial, \Lambda] = -i\bar{\partial}^\*, \quad [\bar{\partial}, \Lambda] = i\partial^\*, \quad [\partial^\*, L] = -i\bar{\partial}, \quad [\bar{\partial}^\*, L] = i\partial.$$ Moreover, we have $$[L, \Lambda] = p + q - n$$ on $A_\mathrm{c}^{p,q}(M)$. 
> *Proof:* Let us first consider the case when $M = \mathbb{C}^n$. Define operators $e_j$ and $\bar{e}\_j$ on $A_\mathrm{c}(M)$ by $$e_j(\alpha) = \mathrm{d}z^j \wedge \alpha, \quad \bar{e}\_j(\alpha) = \mathrm{d}\bar{z}^j \wedge \alpha, \quad \alpha \in A_\mathrm{c}(M), \quad j = 1, \cdots, n.$$ We see that $e_j$ and $\bar{e}\_j$ are $C^\infty(\mathbb{C}^n)$-linear, and hence we may consider their dual operators $l_j$ and $\bar{l}\_j$. The following anti-commutative relations is clear from our definition: $$e_j e_k = -e_k e_j, \quad e_j \bar{e}\_k = -\bar{e}\_k e_j, \quad \bar{e}\_j \bar{e}\_k = -\bar{e}\_k \bar{e}\_j,$$ $$l_j l_k = -l_k l_j, \quad l_j \bar{l}\_k = -\bar{l}\_k l_j, \quad \bar{l}\_j \bar{l}\_k = -\bar{l}\_k \bar{l}\_j,$$ Define operators $\partial_j$ and $\bar{\partial}\_j$ on $A_\mathrm{c}(M)$ by $$\partial_j(f \\\, \mathrm{d}z^I \wedge \mathrm{d}\bar{z}^J) = \frac{\partial f}{\partial z^j} \mathrm{d}z^I \wedge \mathrm{d}\bar{z}^J, \quad \bar{\partial}\_j(f \\\, \mathrm{d}z^I \wedge \mathrm{d}\bar{z}^J) = \frac{\partial f}{\partial \bar{z}^j} \mathrm{d}z^I \wedge \mathrm{d}\bar{z}^J, \quad f \in C^\infty_\mathrm{c}(M), \quad I, J \subset \\\{1, \cdots, n\\\}.$$ It is direct to see that $\partial_j$ and $\bar{\partial}\_j$ commute with each $e_k$, $\bar{e}\_k$, $l_k$ and $\bar{l}\_k$. We also have $$\partial = \sum_{j=1}^n \partial_j e_j, \quad \bar{\partial} = \sum_{j=1}^n \bar{\partial}\_j \bar{e}\_j, \quad L = \frac{i}{2}\sum_{j=1}^n e_j \bar{e}\_j, \quad \Lambda = -\frac{i}{2}\sum_{j=1}^n \bar{l}\_j l_j.$$ Note that for each $$\alpha = f \\\, \mathrm{d}z^I \wedge \mathrm{d}\bar{z}^J, \quad \beta = g \\\, \mathrm{d}z^I \wedge \mathrm{d}\bar{z}^J$$ with $|I| = p$ and $|J| = q$, we have $$(\partial_j \alpha, \beta) = 2^{p+q}\int_{\mathbb{C}^n} \partial_j f \cdot \bar{g} \\\, \mathrm{d}V = -2^{p+q}\int_{\mathbb{C}^n} f \cdot \partial_j \bar{g} \\\,\mathrm{d}V = -(\alpha, \bar{\partial}\_j \beta),$$ implying that $\partial_j^\* = -\bar{\partial}\_j$. Similarly we have $\bar{\partial}\_j^\* = -\partial_j$. It follows that $$\partial^\* = \sum_{j=1}^n \partial_j^\* e_j^\* = -\sum_{j=1}^n \bar{\partial}\_j l_j, \quad \bar{\partial}^\* = \sum_{j=1}^n \bar{\partial}\_j^\* \bar{e}\_j^\* = -\sum_{j=1}^n \partial_j \bar{l}\_j.$$
>
> Consider the interaction of $e_j$ and $l_k$. First note that if $k \not\in I$, then $$(l_k(f \\\, \mathrm{d}z^I \wedge \mathrm{d}\bar{z}^J), \alpha) = (f \\\, \mathrm{d}z^I \wedge \mathrm{d}\bar{z}^J, \mathrm{d}z^k \wedge \alpha) = 0$$ holds for any $\alpha \in A_\mathrm{c}(M)$, implying that $$l_k(f \\\, \mathrm{d}z^I \wedge \mathrm{d}\bar{z}^J) = 0, \quad k \not\in I.$$ At the same time, we have $$(l_k(f \\\, \mathrm{d}z^k \wedge \mathrm{d}z^I \wedge \mathrm{d}\bar{z}^J), \alpha) = (f \\\, \mathrm{d}z^k \wedge \mathrm{d}z^I \wedge \mathrm{d}\bar{z}^J, \mathrm{d}z^k \wedge \alpha) = 2(f \\\, \mathrm{d}z^I \wedge \mathrm{d}\bar{z}^J, \alpha),$$ implying that $$l_k(f \\\, \mathrm{d}z^k \wedge \mathrm{d}z^I \wedge \mathrm{d}\bar{z}^J) = 2f \\\, \mathrm{d}z^I \wedge \mathrm{d}\bar{z}^J.$$ It follows that $$l_k e_k(f \\\, \mathrm{d}z^I \wedge \mathrm{d}\bar{z}^J) = \begin{cases} 2f \\\, \mathrm{d}z^I \wedge \mathrm{d}\bar{z}^J, & k \not\in I, \\\\ 0, & k \in I, \end{cases}$$ $$e_k l_k(f \\\, \mathrm{d}z^I \wedge \mathrm{d}\bar{z}^J) = \begin{cases} 0, & k \not\in I, \\\\ 2f \\\, \mathrm{d}z^I \wedge \mathrm{d}\bar{z}^J, & k \in I, \end{cases}$$ which implies that $$l_k e_k + e_k l_k = 2.$$ Now for $j \neq k$, we have $$l_k e_j (f \\\, \mathrm{d}z^k \wedge \mathrm{d}z^I \wedge \mathrm{d}\bar{z}^J) = l_k(f \\\, \mathrm{d}z^j \wedge \mathrm{d}z^k \wedge \mathrm{d}z^I \wedge \mathrm{d}\bar{z}^J) = -2f \\\, \mathrm{d}z^j \wedge \mathrm{d}z^I \wedge \mathrm{d}\bar{z}^J, \quad j \not\in I,$$ $$e_j l_k (f \\\, \mathrm{d}z^k \wedge \mathrm{d}z^I \wedge \mathrm{d}\bar{z}^J) = e_j (2f \\\, \mathrm{d}z^I \wedge \mathrm{d}\bar{z}^J) = 2f \\\, \mathrm{d}z^j \wedge \mathrm{d}z^I \wedge \mathrm{d}\bar{z}^J, \quad j \not\in I,$$ and hence $$(l_k e_j + e_j l_k)(f \\\, \mathrm{d}z^I \wedge \mathrm{d}\bar{z}^J) = 0, \quad j \not\in I, \quad k \in I.$$ Since this also holds when either $j \in I$ or $k \not\in I$, we obtain $$l_k e_j + e_j l_k = 0, \quad j \neq k.$$ By a similar arguments, we see that $$\bar{l}\_k\bar{e}\_k + \bar{e}\_k\bar{l}\_k = 2,$$ and that for $j \neq k$ $$\bar{l}\_k\bar{e}\_j + \bar{e}\_j\bar{l}\_k = 0.$$ Moreover, for any $j$ and $k$, it always holds that $$l_k\bar{e}\_j + \bar{e}\_j l_k = \bar{l}\_k e_j + e_j \bar{l}\_k = 0.$$ Now we can compute that $$[\partial, \Lambda] = -\frac{i}{2}\sum_{j,k=1}^n (\bar{l}\_j l_j \partial_k e_k - \partial_k e_k \bar{l}\_j l_j) = -\frac{i}{2}\sum_{j,k=1}^n \partial_k \bar{l}\_j (l_j e_k + e_k l_j) = -\frac{i}{2}\sum_{j,k=1}^n 2 \delta_{jk} \partial_k \bar{l}\_j = -i \bar{\partial}^\*.$$ Taking conjugation, we obtain $$[\bar{\partial}, \Lambda] = \overline{[\partial, \Lambda]} = i\partial^\*.$$ Moving to the dual operators, it follows that $$[\partial^\*, L] = -[\partial, \Lambda]^\* = -i\bar{\partial}, \quad [\bar{\partial}^\*, L] = -[\bar{\partial}, \Lambda]^\* = i\partial.$$ We also have $$[L, \Lambda] = \frac{1}{4}\sum_{j,k=1}^n (e_j \bar{e}\_j \bar{l}\_k l_k - \bar{l}\_k l_k e_j \bar{e}\_j) = \frac{1}{4}\sum_{j,k=1}^n (2\delta_{jk} e_j l_k - e_j\bar{l}\_k \bar{e}\_j l_k - \bar{l}\_k l_k e_j \bar{e}\_j) = \frac{1}{4}\sum_{j,k=1} [2\delta_{jk} e_j l_k - \bar{l}\_k (e_j l_k + l_k e_j) \bar{e}\_j] = \frac{1}{2}\sum_{j=1}^n (e_j l_j - \bar{l}\_j \bar{e}\_j).$$ For a form $\alpha = f \\\, \mathrm{d}z^I \wedge \mathrm{d}\bar{z}^J \in A_\mathrm{c}^{p,q}(M)$, we have $$\sum_{j=1}^n e_j l_j (\alpha) = \sum_{j \in I} 2f \\\, \mathrm{d}z^I \wedge \mathrm{d}\bar{z}^J = 2p \alpha,$$ $$\sum_{j=1}^n \bar{l}\_j \bar{e}\_j (\alpha) = \sum_{j \not\in J} 2 \\\, \mathrm{d}z^I \wedge \mathrm{d}\bar{z}^J = 2(n - q)\alpha.$$ It follows that $$[L, \Lambda]\alpha = (p + q - n)\alpha, \quad \alpha \in A_\mathrm{c}^{p,q}(M).$$
>
> Now the identities have been proven for $M = \mathbb{C}^n$. For the general cases, we need the local description of a K&#228;hler metric. Consider an arbitrary point $p \in M$. There exists a local orthogonal frame $\varphi^1, \cdots, \varphi^n$ around $p$ such that $\mathrm{d}\varphi^j(p) = 0$ for any $j$. Replacing $\mathrm{d}z^j$ by $\varphi^j$ and doing the same computation, we see that $[\partial, \Lambda]\alpha$ and $-i\bar{\partial}^\*\alpha$ agrees up to some terms involving $\partial\varphi^j$ and $\bar{\partial}\varphi^j$, which vanish at $p$. Using the similar arguments, the above identities all hold at $p$. Since they only involve global operators, we obtain the desired results. 

## Hodge decomposition

Now suppose $M$ is a compact K&#228;hler manifold. Recall that we have the Laplace-Beltrami operators $$\Delta_\mathrm{d} = \mathrm{d}\mathrm{d}^\* + \mathrm{d}^\*\mathrm{d}, \quad \Delta_\partial = \partial\partial^\* + \partial^\*\partial, \quad \Delta_\bar{\partial} = \bar{\partial}\bar{\partial}^\* + \bar{\partial}^\*\bar{\partial}.$$ Denote the spaces of corresponding harmonic forms by $\mathcal{H}\_\mathrm{d}(M)$, $\mathcal{H}\_\partial(M)$ and $\mathcal{H}\_\bar{\partial}(M)$, and let $$\mathcal{H}^r_\bullet(M) = \mathcal{H}\_\bullet(M) \cap A^r(M), \quad \mathcal{H}^{p,q}\_\bullet(M) = \mathcal{H}\_\bullet(M) \cap A^{p,q}(M),$$ where $\bullet$ is $\mathrm{d}, \partial$ or $\bar{\partial}$. By the Hodge theorem, we have the natural isomorphism $$\mathcal{H}^{p,q}\_\bar{\partial}(M) \cong H^{p,q}(M)$$ for each $p$ and $q$. Meanwhile, by the Hodge theory on compact Riemannian manifolds, there is an analogous result that we have the natural isomorphism $$\mathcal{H}^r_\mathrm{d}(M) \cong H^r(M; \mathbb{C})$$ for each $r$. 

**Proposition.** Suppose $M$ is a compact K&#228;hler manifold. Then $$\Delta_\mathrm{d} = 2 \Delta_\partial = 2\Delta_\bar{\partial}.$$

> *Proof:* We will use the fundamental identities we have shown above. Since $\mathrm{d} = \partial + \bar{\partial}$, we have $\mathrm{d}^\* = \partial^\* + \bar{\partial}^\*$, and hence $$\Delta_\mathrm{d} = (\partial\partial^\* + \partial\bar{\partial}^\* + \bar{\partial}\partial^\* + \bar{\partial}\bar{\partial}^\*) + (\partial^\*\partial + \partial^\*\bar{\partial} + \bar{\partial}^\*\partial + \bar{\partial}^\*\bar{\partial}) = \Delta_\partial + \Delta_\bar{\partial} + (\partial\bar{\partial}^\* + \bar{\partial}^\*\partial) + (\bar{\partial}\partial^\* + \partial^\*\bar{\partial}).$$ Since $\bar{\partial}^\* = i[\partial, \Lambda]$ and $\partial^\* = -i[\bar{\partial}, \Lambda]$, we obtain $$\partial\bar{\partial}^\* + \bar{\partial}^\*\partial = i(\partial[\partial, \Lambda] + [\partial, \Lambda]\partial) = i[\partial^2, \Lambda] = 0,$$ $$\bar{\partial}\partial^\* + \partial^\*\bar{\partial} = -i(\bar{\partial}[\bar{\partial}, \Lambda] + [\bar{\partial}, \Lambda]\bar{\partial}) = -i[\bar{\partial}^2, \Lambda] = 0.$$ It follows that $$\Delta_\mathrm{d} = \Delta_\partial + \Delta_\bar{\partial}.$$ Hence it remains to show that $\Delta_\partial = \Delta_\bar{\partial}$. Direct computation yields that $$\Delta_\partial - \Delta_\bar{\partial} = -i(\partial[\bar{\partial}, \Lambda] + [\bar{\partial}, \Lambda]\partial + \bar{\partial}[\partial, \Lambda] + [\partial, \Lambda]\bar{\partial}) = -i[\partial\bar{\partial} + \bar{\partial}\partial, \Lambda] = 0.$$

This relations of $\Delta_\mathrm{d}$, $\Delta_\partial$ and $\Delta_\bar{\partial}$ implies that $$\mathcal{H}\_\mathrm{d}(M) = \mathcal{H}\_\partial(M) = \mathcal{H}\_\bar{\partial}(M),$$ and hence we may simply denote them by $\mathcal{H}(M)$. Since $\Delta_\mathrm{d}$ is clearly a real operator, we see that for $\alpha \in A^{p,q}(M)$, $$\alpha \in \mathcal{H}^{p,q}(M) \iff \Delta_\mathrm{d}\alpha = 0 \iff \Delta_\mathrm{d}\bar{\alpha} = 0 \iff \bar{\alpha} \in \mathcal{H}^{q,p}(M),$$ implying that $$\overline{\mathcal{H}^{p,q}(M)} = \mathcal{H}^{q,p}(M).$$ Moreover, for a harmonic $\alpha \in \mathcal{H}^r(M)$, we can decompose it into $$\alpha = \sum_{p+q=r} \alpha^{p,q}, \quad \alpha^{p,q} \in A^{p,q}(M).$$ Then $$0 = \Delta_\bar{\partial}\alpha = \sum_{p+q=r} \Delta_\bar{\partial}\alpha^{p,q},$$ with $\Delta_\bar{\partial}\alpha^{p,q} \in A^{p,q}(M)$. Using the uniqueness of the decomposition of $r$-forms, we see that $\Delta_\bar{\partial}\alpha^{p,q} = 0$ and hence $\alpha^{p,q} \in \mathcal{H}^{p,q}(M)$. It then follows that we have the direct sum decompostion of spaces $$\mathcal{H}^r(M) = \bigoplus_{p+q=r} \mathcal{H}^{p,q}(M).$$ Passing this to the cohomology, we obtain the Hodge decompostion.

**Theorem (Hodge decomposition).** Suppose $M$ is a compact K&#228;hler manifold, then for each $0 \leq r \leq 2n$, we have the decomposition $$H^r(M; \mathbb{C}) \cong \bigoplus_{p+q=r} H^{p,q}(M).$$ Under this isomorphism, each $H^{p,q}(M)$ is identified with a subspace of $H^r(M; \mathbb{C})$, through which we have $$\overline{H^{p,q}(M)} = H^{q,p}(M), \quad p + q = r.$$

Recall that we have the Betti numbers $$b_r(M) = \dim H^r(M; \mathbb{C}), \quad 0 \leq r \leq 2n.$$ Similarly, we define the **Hodge numbers** $h^{p,q}$ by $$h^{p,q}(M) = \dim H^{p,q}(M), \quad 0 \leq p,q \leq n.$$ By the above Hodge decomposition theorem, we have the relations between Betti numbers and Hodge numbers given as $$b_r = \sum_{p+q=r} h^{p,q}, \quad 0 \leq r \leq 2n; \quad h^{p,q} = h^{q,p}, \quad 0 \leq p, q \leq n.$$ A direct consequence is that $b_{2k-1}$ must be even as we have $$b_{2k-1} = \sum_{p+q=2k-1} h^{p,q} = 2 \sum_{p=0}^{k-1} h^{p,2k-1-p}.$$ Thus there is a topological constraint for a manifold to be K&#228;hler, that is *the Betti numbers of odd order should be even, and the Betti numbers of even order should be positive.*

We may apply the above results to compute the Dolbeault cohomology of $\mathbb{P}^n$. 

**Proposition.** The Dolbeault cohomology groups of $\mathbb{P}^n$ is given by $$H^{p,q}(\mathbb{P}^n) = \begin{cases} \mathbb{C}, & 0 \leq p = q \leq n; \\\\ 0 & \text{otherwise}.\end{cases}$$

> *Proof:* The assertion is equivalent to that $$h^{p,q} = \begin{cases} 1, & 0 \leq p = q \leq n; \\\\ 0 & \text{otherwise}.\end{cases}$$ Note that by the singular cohomology, we have $$b_{2k} = 1, \quad 0 \leq k \leq 1; \quad b_{2k-1} = 0.$$ If we have any $h^{p,q} > 0$ with $p \neq q$, then $$b_{p+q} \geq h^{p,q} + h^{q,p} \geq 2,$$ a contradiction. Hence we must have $h^{p,p} = 1$ for each $1 \leq p \leq n$ and $h^{p,q} = 0$ for other cases. 